\documentclass[a4j,twocolumn]{jarticle}

%% プリアンブル部 %%
\usepackage{fancybox}
\usepackage{ascmac}
\usepackage{amsmath}
 

\begin{document}

\title{数式演習}
\author{Christian Harjuno}
\date{2024年4月28日}

\maketitle
\thispagestyle{empty}

\begin{equation}
x_{10}=a^5+b^{11}+\sqrt{c} 
\end{equation}

\begin{equation}
x = a + b - c \times d \div e
\end{equation}

\begin{equation}
\sqrt[8]{a + b}
\end{equation}

\begin{equation}
m\vec{a} = \vec{F}
\end{equation}

\begin{equation}
y = x^{4n} + 3x^{2n-1} + 2x - 1
\end{equation}

\begin{equation}
x = \frac{-b \pm \sqrt{b^2 - 4ac}}{2a}
\end{equation}

\begin{equation}
\forall x \in A,\exists x > 0
\end{equation}

\begin{equation}
\Delta ABC \equiv \Delta DEF
\end{equation}

\begin{equation}
\sum_{i = 1}^{n}i = 1 + 2 + \cdots + n = \frac{n(n + 1)}{2}
\end{equation}

\begin{equation}
\vec{a} \cdot \vec{b} = \left| \vec{a} \right| \left| \vec{b} \right| \cos \theta 
\end{equation}

\begin{equation}
  _n{C}_k = \frac{n!}{k!(n - k)!} \neq \infty
\end{equation}

\begin{equation}
  x = \text{second\_max}\left\{a_1,a_2,a_3,\cdot a_n\right\}
\end{equation}

\begin{equation}
  y = \sqrt{3x} \log x
\end{equation}

\begin{equation}
  \sin (\alpha - \beta) = \sin \alpha \cos \beta - \cos \alpha \sin \beta
\end{equation}

\begin{equation}
  p = \max\left\{\ k | p_k \in X,s_k \notin Y,1\leq k\leq n \right\}
\end{equation}

\begin{equation}
  \overline{p + q} = \bar{p} \cdot \bar{q}
\end{equation}

\begin{equation}
  p \wedge \bar{q} = \overline{p \rightarrow q}
\end{equation}

\begin{equation}
  P \subset Q, P\subseteq Q
\end{equation}

\begin{equation}
  P \cap Q = \emptyset, P \cup Q \neq \emptyset
\end{equation}

\begin{equation}
  \left( {p \Rightarrow q }\right) \wedge \left( {p \Leftarrow q }\right) \equiv p \Leftrightarrow q
\end{equation}

\begin{equation}
  a = \lim_{x \rightarrow \infty} f\left(x\right)
\end{equation}

\begin{equation}
  \int_{x=2}^{4} \cot x\log xdx
\end{equation}

\begin{equation}
  \begin{pmatrix}
    3 & 2 & 1\\
    2 & 1 & 3\\
    1 & 2 & 3\\
  \end{pmatrix}
\end{equation}

\begin{equation}
  F(n) = \left\{
    \begin{aligned}
      n \times F(n - 1) & \quad (n > 1) \\
      1 & \quad  (n = 0)
    \end{aligned}
  \right.
\end{equation}


\begin{equation}
  \begin{aligned}
    {(a - b)}^3 &= (a-b){(a-b)}^2 \\
    &= (a - b)(a^2 - 2ab + b^2)\\ 
    &= a^3 - 3a^2b + 3ab^2 - b^3

  \end{aligned}
\end{equation}


\end{document}